lazy_list/spec.v
@@ -1,0 +1,65 @@
+From iris.heap_lang Require Import notation proofmode.
+From iris.base_logic.lib Require Export invariants.
+
+From SkipList.lazy_list Require Import code.
+
+From Coq Require Import Lists.ListSet.
+
+Local Open Scope Z.
+Module LazyListSpec (Params: LAZYLIST_PARAMS).
+  Import Params.
+  Module Code := Lazylist Params.
+  Export Code.
+
+Context `{!heapGS Σ} (N : namespace).
+
+Fixpoint list_equiv (L: list Z) (node: val) : iProp Σ :=
+  match L with
+  | nil => ⌜ node = NONEV ⌝
+  | h :: t => ∃ (k: Z) (n: loc) (m: bool) (l: val) (v': val) (γ: gname),
+              ⌜ node = rep_to_node (k, n, m, l) ⌝
+              ∗
+              n ↦ v'
+              ∗
+              (* is_lock γ l ???
+              ∗ *)
+              list_equiv t v'
+  end.
+
+Definition lazy_list_inv (S: set Z) (l: loc) : iProp Σ := 
+  ∃ (L: list Z) (head: val),
+  (* ⌜ Permutation L (elements S) ⌝
+  ∗ *)
+  (* ⌜ Sorted Zlt L ⌝
+  ∗ *)
+  l ↦ head
+  ∗
+  list_equiv L head
+.
+
+Definition is_lazy_list (S: set Z) (l: loc) : iProp Σ := 
+  inv N (lazy_list_inv S l).
+
+Definition empty_lazy := [INT_MIN; INT_MAX].
+
+Theorem new_spec :
+  {{{ True }}}
+    new #()
+  {{{ l, RET l; 
+    is_lazy_list empty_lazy l 
+  }}}.
+Proof.
+Admitted.
+
+Theorem contains_spec (S: set Z) (l: loc) (key: Z) :
+  {{{ is_lazy_list S l }}}
+    contains !#l #key
+  {{{ b, RET b; 
+    is_lazy_list S l
+    ∗
+    ⌜ (b = False ∧ ¬ key ∈ S)
+    ∨
+    (b = True ∧ key ∈ S) ⌝
+  }}}.
+Proof.
+Admitted.
